moving to homogeneous equalities

examples/refinement/Example1.fst
@@ -10,33 +10,79 @@ effect Hi (a:Type)
           (post: HighComp.state -> a -> HighComp.state -> Type) =
        HighMon a (fun s0 k -> pre s0  /\ (forall x s1. post s0 x s1 ==> k (x, s1)))
 
-effect HTot (a:Type) = Hi a (fun _ -> True) (fun _ _ _ -> True)
-
 let morph #a (#wp:H.hwp_mon a) ($c:H.HIGH?.repr a wp) : L.lcomp_wp a wp c =
    L.morph #a wp c
 
-let test_return () : HTot bool = true
-let low_return () : L.lcomp_wp bool _ _ = morph (reify (test_return ()))
+// let low_return () : L.lcomp_wp bool _ _ = morph (reify (test_return ()))
 
 open FStar.Tactics
-assume val eq_any : #a:Type -> #b:Type -> x:a -> y:b -> Lemma (x === y)
-let test (a:Type) (wp:H.hwp_mon a) (c:H.comp_wp a wp) =
-    assert (L.morph wp c === L.lreturn true)
-        by (dump "A"; apply_lemma (`L.morph_return); dump "B")
+
+effect HTot (a:Type) = HighComp.HIGH a (fun s post -> forall x. post x)
+let test_return () : HTot bool = true
+// assume val eq_any : #a:Type -> #b:Type -> x:a -> y:b -> Lemma (x === y)
+// #set-options "--debug Example1 --debug_level Rel"
+// let test =
+//     assert (reify (test_return ()) === H.return_elab true)
+//         by (apply_lemma (`eq_any))
 
 
-let sum_and_swap () : Hi uint_32
-    (requires (fun (x0, x1) -> ok (+) x0 x1))
-    (ensures (fun _ _ _ -> True)) =
-   let x0 = H.get_action 0 in
-   let x1 = H.get_action 1 in
-   H.put_action 0 x1;
-   H.put_action 1 x0;
-   x0 + x1
+let test =
+    assert (LowComp.morph #_ _ (H.return_elab true) == L.lreturn true)
+        by (dump "A"; apply_lemma (`L.morph_return); dump "B") //spawns SMT proof of monotonicity
 
-let test = reify (sum_and_swap ())
-let x = HighComp.HIGH?.repr
+let test2 =
+    assert (LowComp.morph #_ _ (H.hread_elab 0) == L.lread' 0)
+        by (apply_lemma (`L.morph_read))
+
+let test3 (#a:Type0) (#b:Type0)
+          (#wpa:H.hwp_mon a) (#wpb: (a -> H.hwp_mon b))
+          (c1:H.comp_wp a wpa) (c2: (x:a -> H.comp_wp b (wpb x))) =
+    assert (LowComp.morph #_ _ (H.bind_elab c1 c2) == L.lbind (morph c1) (fun x -> morph (c2 x)))
+        by (apply_lemma (`L.morph_bind))
+
+open FStar.FunctionalExtensionality
 
 
+let apply_feq2_lem #a #b #c ($f $g : a -> b -> c) : Lemma (requires (forall x y. f x y == g x y))
+                                                        (ensures (f == g)) =
+    assert (forall x. feq (f x) (g x));
+    assert (feq f g)
 
-let test2 = morph (reify (sum_and_swap ()))
+
+let apply_feq_lem #a #b ($f $g : a -> b) : Lemma (requires (forall x. f x == g x))
+                                                (ensures (f == g)) =
+    assert (feq f g)
+
+let fext () = apply_lemma (`apply_feq_lem); dismiss (); ignore (forall_intros ())
+
+let morph_bind () = dump "A"; fext (); dump "B"; apply_lemma (`L.morph_bind)
+
+#set-options "--debug Example1 --debug_level Rel"
+//[@(postprocess_with morph_bind)]
+let test4 (#a:Type0)
+          (#b:Type0)
+          (#wpa:H.hwp_mon a)
+          (#wpb: (a -> H.hwp_mon b))
+          (c1:H.comp_wp a wpa)
+           =
+    assert ((fun (c2: (x:a -> H.comp_wp b (wpb x))) ->
+              LowComp.morph #b (H.bind_wp wpa wpb) (H.bind_elab c1 c2)) ==
+            (fun (c2: (x:a -> H.comp_wp b (wpb x))) -> L.lbind (morph c1) (fun x -> morph (c2 x))))
+       by (dump "A"; fext(); dump "B")
+
+    // assert (morph (H.bind_elab c1 c2) === L.lbind (morph c1) (fun x -> morph (c2 x)))
+    //     by (apply_lemma (`L.morph_bind))
+
+// let swap : comp_wp unit _ =
+//   bind_elab (get_action 0) (fun x0 0
+
+// let sum_and_swap () : Hi uint_32
+//     (requires (fun (x0, x1) -> ok (+) x0 x1))
+//     (ensures (fun _ _ _ -> True)) =
+//    let x0 = H.get_action 0 in
+//    let x1 = H.get_action 1 in
+//    H.put_action 0 x1;
+//    H.put_action 1 x0;
+//    x0 + x1
+
+// // let test2 = morph (reify (sum_and_swap ()))
